theories/Autosubst2/syntax.v
@@ -5,118 +5,88 @@ Require Import Setoid Morphisms Relation_Definitions.
 
 Module Core.
 
-Inductive Sort : Type :=
-  | Kind : Sort
-  | Star : Sort.
-
-Lemma congr_Kind : Kind = Kind.
-Proof.
-exact (eq_refl).
-Qed.
+Inductive Ki : Type :=
+  | Star : Ki
+  | Arr : Ki -> Ki -> Ki.
 
 Lemma congr_Star : Star = Star.
 Proof.
 exact (eq_refl).
 Qed.
 
-Inductive Term : Type :=
-  | VarTm : nat -> Term
-  | ISort : Sort -> Term
-  | Abs : Term -> Term -> Term
-  | App : Term -> Term -> Term
-  | Pi : Term -> Term -> Term.
-
-Lemma congr_ISort {s0 : Sort} {t0 : Sort} (H0 : s0 = t0) :
-  ISort s0 = ISort t0.
+Lemma congr_Arr {s0 : Ki} {s1 : Ki} {t0 : Ki} {t1 : Ki} (H0 : s0 = t0)
+  (H1 : s1 = t1) : Arr s0 s1 = Arr t0 t1.
 Proof.
-exact (eq_trans eq_refl (ap (fun x => ISort x) H0)).
+exact (eq_trans (eq_trans eq_refl (ap (fun x => Arr x s1) H0))
+         (ap (fun x => Arr t0 x) H1)).
 Qed.
 
-Lemma congr_Abs {s0 : Term} {s1 : Term} {t0 : Term} {t1 : Term}
-  (H0 : s0 = t0) (H1 : s1 = t1) : Abs s0 s1 = Abs t0 t1.
+Inductive Tm : Type :=
+  | VarTm : nat -> Tm
+  | TmAbs : Tm -> Tm
+  | TmApp : Tm -> Tm -> Tm.
+
+Lemma congr_TmAbs {s0 : Tm} {t0 : Tm} (H0 : s0 = t0) : TmAbs s0 = TmAbs t0.
 Proof.
-exact (eq_trans (eq_trans eq_refl (ap (fun x => Abs x s1) H0))
-         (ap (fun x => Abs t0 x) H1)).
+exact (eq_trans eq_refl (ap (fun x => TmAbs x) H0)).
 Qed.
 
-Lemma congr_App {s0 : Term} {s1 : Term} {t0 : Term} {t1 : Term}
-  (H0 : s0 = t0) (H1 : s1 = t1) : App s0 s1 = App t0 t1.
+Lemma congr_TmApp {s0 : Tm} {s1 : Tm} {t0 : Tm} {t1 : Tm} (H0 : s0 = t0)
+  (H1 : s1 = t1) : TmApp s0 s1 = TmApp t0 t1.
 Proof.
-exact (eq_trans (eq_trans eq_refl (ap (fun x => App x s1) H0))
-         (ap (fun x => App t0 x) H1)).
+exact (eq_trans (eq_trans eq_refl (ap (fun x => TmApp x s1) H0))
+         (ap (fun x => TmApp t0 x) H1)).
 Qed.
 
-Lemma congr_Pi {s0 : Term} {s1 : Term} {t0 : Term} {t1 : Term} (H0 : s0 = t0)
-  (H1 : s1 = t1) : Pi s0 s1 = Pi t0 t1.
-Proof.
-exact (eq_trans (eq_trans eq_refl (ap (fun x => Pi x s1) H0))
-         (ap (fun x => Pi t0 x) H1)).
-Qed.
-
-Lemma upRen_Term_Term (xi : nat -> nat) : nat -> nat.
+Lemma upRen_Tm_Tm (xi : nat -> nat) : nat -> nat.
 Proof.
 exact (up_ren xi).
 Defined.
 
-Fixpoint ren_Term (xi_Term : nat -> nat) (s : Term) {struct s} : Term :=
+Fixpoint ren_Tm (xi_Tm : nat -> nat) (s : Tm) {struct s} : Tm :=
   match s with
-  | VarTm s0 => VarTm (xi_Term s0)
-  | ISort s0 => ISort s0
-  | Abs s0 s1 =>
-      Abs (ren_Term xi_Term s0) (ren_Term (upRen_Term_Term xi_Term) s1)
-  | App s0 s1 => App (ren_Term xi_Term s0) (ren_Term xi_Term s1)
-  | Pi s0 s1 =>
-      Pi (ren_Term xi_Term s0) (ren_Term (upRen_Term_Term xi_Term) s1)
+  | VarTm s0 => VarTm (xi_Tm s0)
+  | TmAbs s0 => TmAbs (ren_Tm (upRen_Tm_Tm xi_Tm) s0)
+  | TmApp s0 s1 => TmApp (ren_Tm xi_Tm s0) (ren_Tm xi_Tm s1)
   end.
 
-Lemma up_Term_Term (sigma : nat -> Term) : nat -> Term.
+Lemma up_Tm_Tm (sigma : nat -> Tm) : nat -> Tm.
 Proof.
-exact (scons (VarTm var_zero) (funcomp (ren_Term shift) sigma)).
+exact (scons (VarTm var_zero) (funcomp (ren_Tm shift) sigma)).
 Defined.
 
-Fixpoint subst_Term (sigma_Term : nat -> Term) (s : Term) {struct s} : 
-Term :=
+Fixpoint subst_Tm (sigma_Tm : nat -> Tm) (s : Tm) {struct s} : Tm :=
   match s with
-  | VarTm s0 => sigma_Term s0
-  | ISort s0 => ISort s0
-  | Abs s0 s1 =>
-      Abs (subst_Term sigma_Term s0)
-        (subst_Term (up_Term_Term sigma_Term) s1)
-  | App s0 s1 => App (subst_Term sigma_Term s0) (subst_Term sigma_Term s1)
-  | Pi s0 s1 =>
-      Pi (subst_Term sigma_Term s0) (subst_Term (up_Term_Term sigma_Term) s1)
+  | VarTm s0 => sigma_Tm s0
+  | TmAbs s0 => TmAbs (subst_Tm (up_Tm_Tm sigma_Tm) s0)
+  | TmApp s0 s1 => TmApp (subst_Tm sigma_Tm s0) (subst_Tm sigma_Tm s1)
   end.
 
-Lemma upId_Term_Term (sigma : nat -> Term) (Eq : forall x, sigma x = VarTm x)
-  : forall x, up_Term_Term sigma x = VarTm x.
+Lemma upId_Tm_Tm (sigma : nat -> Tm) (Eq : forall x, sigma x = VarTm x) :
+  forall x, up_Tm_Tm sigma x = VarTm x.
 Proof.
 exact (fun n =>
        match n with
-       | S n' => ap (ren_Term shift) (Eq n')
+       | S n' => ap (ren_Tm shift) (Eq n')
        | O => eq_refl
        end).
 Qed.
 
-Fixpoint idSubst_Term (sigma_Term : nat -> Term)
-(Eq_Term : forall x, sigma_Term x = VarTm x) (s : Term) {struct s} :
-subst_Term sigma_Term s = s :=
+Fixpoint idSubst_Tm (sigma_Tm : nat -> Tm)
+(Eq_Tm : forall x, sigma_Tm x = VarTm x) (s : Tm) {struct s} :
+subst_Tm sigma_Tm s = s :=
   match s with
-  | VarTm s0 => Eq_Term s0
-  | ISort s0 => congr_ISort (eq_refl s0)
-  | Abs s0 s1 =>
-      congr_Abs (idSubst_Term sigma_Term Eq_Term s0)
-        (idSubst_Term (up_Term_Term sigma_Term) (upId_Term_Term _ Eq_Term) s1)
-  | App s0 s1 =>
-      congr_App (idSubst_Term sigma_Term Eq_Term s0)
-        (idSubst_Term sigma_Term Eq_Term s1)
-  | Pi s0 s1 =>
-      congr_Pi (idSubst_Term sigma_Term Eq_Term s0)
-        (idSubst_Term (up_Term_Term sigma_Term) (upId_Term_Term _ Eq_Term) s1)
+  | VarTm s0 => Eq_Tm s0
+  | TmAbs s0 =>
+      congr_TmAbs (idSubst_Tm (up_Tm_Tm sigma_Tm) (upId_Tm_Tm _ Eq_Tm) s0)
+  | TmApp s0 s1 =>
+      congr_TmApp (idSubst_Tm sigma_Tm Eq_Tm s0)
+        (idSubst_Tm sigma_Tm Eq_Tm s1)
   end.
 
-Lemma upExtRen_Term_Term (xi : nat -> nat) (zeta : nat -> nat)
+Lemma upExtRen_Tm_Tm (xi : nat -> nat) (zeta : nat -> nat)
   (Eq : forall x, xi x = zeta x) :
-  forall x, upRen_Term_Term xi x = upRen_Term_Term zeta x.
+  forall x, upRen_Tm_Tm xi x = upRen_Tm_Tm zeta x.
 Proof.
 exact (fun n => match n with
                 | S n' => ap shift (Eq n')
@@ -124,497 +94,891 @@ exact (fun n => match n with
                 end).
 Qed.
 
-Fixpoint extRen_Term (xi_Term : nat -> nat) (zeta_Term : nat -> nat)
-(Eq_Term : forall x, xi_Term x = zeta_Term x) (s : Term) {struct s} :
-ren_Term xi_Term s = ren_Term zeta_Term s :=
+Fixpoint extRen_Tm (xi_Tm : nat -> nat) (zeta_Tm : nat -> nat)
+(Eq_Tm : forall x, xi_Tm x = zeta_Tm x) (s : Tm) {struct s} :
+ren_Tm xi_Tm s = ren_Tm zeta_Tm s :=
   match s with
-  | VarTm s0 => ap (VarTm) (Eq_Term s0)
-  | ISort s0 => congr_ISort (eq_refl s0)
-  | Abs s0 s1 =>
-      congr_Abs (extRen_Term xi_Term zeta_Term Eq_Term s0)
-        (extRen_Term (upRen_Term_Term xi_Term) (upRen_Term_Term zeta_Term)
-           (upExtRen_Term_Term _ _ Eq_Term) s1)
-  | App s0 s1 =>
-      congr_App (extRen_Term xi_Term zeta_Term Eq_Term s0)
-        (extRen_Term xi_Term zeta_Term Eq_Term s1)
-  | Pi s0 s1 =>
-      congr_Pi (extRen_Term xi_Term zeta_Term Eq_Term s0)
-        (extRen_Term (upRen_Term_Term xi_Term) (upRen_Term_Term zeta_Term)
-           (upExtRen_Term_Term _ _ Eq_Term) s1)
+  | VarTm s0 => ap (VarTm) (Eq_Tm s0)
+  | TmAbs s0 =>
+      congr_TmAbs
+        (extRen_Tm (upRen_Tm_Tm xi_Tm) (upRen_Tm_Tm zeta_Tm)
+           (upExtRen_Tm_Tm _ _ Eq_Tm) s0)
+  | TmApp s0 s1 =>
+      congr_TmApp (extRen_Tm xi_Tm zeta_Tm Eq_Tm s0)
+        (extRen_Tm xi_Tm zeta_Tm Eq_Tm s1)
   end.
 
-Lemma upExt_Term_Term (sigma : nat -> Term) (tau : nat -> Term)
+Lemma upExt_Tm_Tm (sigma : nat -> Tm) (tau : nat -> Tm)
   (Eq : forall x, sigma x = tau x) :
-  forall x, up_Term_Term sigma x = up_Term_Term tau x.
+  forall x, up_Tm_Tm sigma x = up_Tm_Tm tau x.
 Proof.
 exact (fun n =>
        match n with
-       | S n' => ap (ren_Term shift) (Eq n')
+       | S n' => ap (ren_Tm shift) (Eq n')
        | O => eq_refl
        end).
 Qed.
 
-Fixpoint ext_Term (sigma_Term : nat -> Term) (tau_Term : nat -> Term)
-(Eq_Term : forall x, sigma_Term x = tau_Term x) (s : Term) {struct s} :
-subst_Term sigma_Term s = subst_Term tau_Term s :=
+Fixpoint ext_Tm (sigma_Tm : nat -> Tm) (tau_Tm : nat -> Tm)
+(Eq_Tm : forall x, sigma_Tm x = tau_Tm x) (s : Tm) {struct s} :
+subst_Tm sigma_Tm s = subst_Tm tau_Tm s :=
   match s with
-  | VarTm s0 => Eq_Term s0
-  | ISort s0 => congr_ISort (eq_refl s0)
-  | Abs s0 s1 =>
-      congr_Abs (ext_Term sigma_Term tau_Term Eq_Term s0)
-        (ext_Term (up_Term_Term sigma_Term) (up_Term_Term tau_Term)
-           (upExt_Term_Term _ _ Eq_Term) s1)
-  | App s0 s1 =>
-      congr_App (ext_Term sigma_Term tau_Term Eq_Term s0)
-        (ext_Term sigma_Term tau_Term Eq_Term s1)
-  | Pi s0 s1 =>
-      congr_Pi (ext_Term sigma_Term tau_Term Eq_Term s0)
-        (ext_Term (up_Term_Term sigma_Term) (up_Term_Term tau_Term)
-           (upExt_Term_Term _ _ Eq_Term) s1)
+  | VarTm s0 => Eq_Tm s0
+  | TmAbs s0 =>
+      congr_TmAbs
+        (ext_Tm (up_Tm_Tm sigma_Tm) (up_Tm_Tm tau_Tm) (upExt_Tm_Tm _ _ Eq_Tm)
+           s0)
+  | TmApp s0 s1 =>
+      congr_TmApp (ext_Tm sigma_Tm tau_Tm Eq_Tm s0)
+        (ext_Tm sigma_Tm tau_Tm Eq_Tm s1)
   end.
 
-Lemma up_ren_ren_Term_Term (xi : nat -> nat) (zeta : nat -> nat)
+Lemma up_ren_ren_Tm_Tm (xi : nat -> nat) (zeta : nat -> nat)
   (rho : nat -> nat) (Eq : forall x, funcomp zeta xi x = rho x) :
-  forall x,
-  funcomp (upRen_Term_Term zeta) (upRen_Term_Term xi) x =
-  upRen_Term_Term rho x.
+  forall x, funcomp (upRen_Tm_Tm zeta) (upRen_Tm_Tm xi) x = upRen_Tm_Tm rho x.
 Proof.
 exact (up_ren_ren xi zeta rho Eq).
 Qed.
 
-Fixpoint compRenRen_Term (xi_Term : nat -> nat) (zeta_Term : nat -> nat)
-(rho_Term : nat -> nat)
-(Eq_Term : forall x, funcomp zeta_Term xi_Term x = rho_Term x) (s : Term)
-{struct s} : ren_Term zeta_Term (ren_Term xi_Term s) = ren_Term rho_Term s :=
+Fixpoint compRenRen_Tm (xi_Tm : nat -> nat) (zeta_Tm : nat -> nat)
+(rho_Tm : nat -> nat) (Eq_Tm : forall x, funcomp zeta_Tm xi_Tm x = rho_Tm x)
+(s : Tm) {struct s} : ren_Tm zeta_Tm (ren_Tm xi_Tm s) = ren_Tm rho_Tm s :=
   match s with
-  | VarTm s0 => ap (VarTm) (Eq_Term s0)
-  | ISort s0 => congr_ISort (eq_refl s0)
-  | Abs s0 s1 =>
-      congr_Abs (compRenRen_Term xi_Term zeta_Term rho_Term Eq_Term s0)
-        (compRenRen_Term (upRen_Term_Term xi_Term)
-           (upRen_Term_Term zeta_Term) (upRen_Term_Term rho_Term)
-           (up_ren_ren _ _ _ Eq_Term) s1)
-  | App s0 s1 =>
-      congr_App (compRenRen_Term xi_Term zeta_Term rho_Term Eq_Term s0)
-        (compRenRen_Term xi_Term zeta_Term rho_Term Eq_Term s1)
-  | Pi s0 s1 =>
-      congr_Pi (compRenRen_Term xi_Term zeta_Term rho_Term Eq_Term s0)
-        (compRenRen_Term (upRen_Term_Term xi_Term)
-           (upRen_Term_Term zeta_Term) (upRen_Term_Term rho_Term)
-           (up_ren_ren _ _ _ Eq_Term) s1)
+  | VarTm s0 => ap (VarTm) (Eq_Tm s0)
+  | TmAbs s0 =>
+      congr_TmAbs
+        (compRenRen_Tm (upRen_Tm_Tm xi_Tm) (upRen_Tm_Tm zeta_Tm)
+           (upRen_Tm_Tm rho_Tm) (up_ren_ren _ _ _ Eq_Tm) s0)
+  | TmApp s0 s1 =>
+      congr_TmApp (compRenRen_Tm xi_Tm zeta_Tm rho_Tm Eq_Tm s0)
+        (compRenRen_Tm xi_Tm zeta_Tm rho_Tm Eq_Tm s1)
   end.
 
-Lemma up_ren_subst_Term_Term (xi : nat -> nat) (tau : nat -> Term)
-  (theta : nat -> Term) (Eq : forall x, funcomp tau xi x = theta x) :
-  forall x,
-  funcomp (up_Term_Term tau) (upRen_Term_Term xi) x = up_Term_Term theta x.
+Lemma up_ren_subst_Tm_Tm (xi : nat -> nat) (tau : nat -> Tm)
+  (theta : nat -> Tm) (Eq : forall x, funcomp tau xi x = theta x) :
+  forall x, funcomp (up_Tm_Tm tau) (upRen_Tm_Tm xi) x = up_Tm_Tm theta x.
 Proof.
 exact (fun n =>
        match n with
-       | S n' => ap (ren_Term shift) (Eq n')
+       | S n' => ap (ren_Tm shift) (Eq n')
        | O => eq_refl
        end).
 Qed.
 
-Fixpoint compRenSubst_Term (xi_Term : nat -> nat) (tau_Term : nat -> Term)
-(theta_Term : nat -> Term)
-(Eq_Term : forall x, funcomp tau_Term xi_Term x = theta_Term x) (s : Term)
-{struct s} :
-subst_Term tau_Term (ren_Term xi_Term s) = subst_Term theta_Term s :=
+Fixpoint compRenSubst_Tm (xi_Tm : nat -> nat) (tau_Tm : nat -> Tm)
+(theta_Tm : nat -> Tm)
+(Eq_Tm : forall x, funcomp tau_Tm xi_Tm x = theta_Tm x) (s : Tm) {struct s} :
+subst_Tm tau_Tm (ren_Tm xi_Tm s) = subst_Tm theta_Tm s :=
   match s with
-  | VarTm s0 => Eq_Term s0
-  | ISort s0 => congr_ISort (eq_refl s0)
-  | Abs s0 s1 =>
-      congr_Abs (compRenSubst_Term xi_Term tau_Term theta_Term Eq_Term s0)
-        (compRenSubst_Term (upRen_Term_Term xi_Term) (up_Term_Term tau_Term)
-           (up_Term_Term theta_Term) (up_ren_subst_Term_Term _ _ _ Eq_Term)
-           s1)
-  | App s0 s1 =>
-      congr_App (compRenSubst_Term xi_Term tau_Term theta_Term Eq_Term s0)
-        (compRenSubst_Term xi_Term tau_Term theta_Term Eq_Term s1)
-  | Pi s0 s1 =>
-      congr_Pi (compRenSubst_Term xi_Term tau_Term theta_Term Eq_Term s0)
-        (compRenSubst_Term (upRen_Term_Term xi_Term) (up_Term_Term tau_Term)
-           (up_Term_Term theta_Term) (up_ren_subst_Term_Term _ _ _ Eq_Term)
-           s1)
+  | VarTm s0 => Eq_Tm s0
+  | TmAbs s0 =>
+      congr_TmAbs
+        (compRenSubst_Tm (upRen_Tm_Tm xi_Tm) (up_Tm_Tm tau_Tm)
+           (up_Tm_Tm theta_Tm) (up_ren_subst_Tm_Tm _ _ _ Eq_Tm) s0)
+  | TmApp s0 s1 =>
+      congr_TmApp (compRenSubst_Tm xi_Tm tau_Tm theta_Tm Eq_Tm s0)
+        (compRenSubst_Tm xi_Tm tau_Tm theta_Tm Eq_Tm s1)
   end.
 
-Lemma up_subst_ren_Term_Term (sigma : nat -> Term) (zeta_Term : nat -> nat)
-  (theta : nat -> Term)
-  (Eq : forall x, funcomp (ren_Term zeta_Term) sigma x = theta x) :
+Lemma up_subst_ren_Tm_Tm (sigma : nat -> Tm) (zeta_Tm : nat -> nat)
+  (theta : nat -> Tm)
+  (Eq : forall x, funcomp (ren_Tm zeta_Tm) sigma x = theta x) :
   forall x,
-  funcomp (ren_Term (upRen_Term_Term zeta_Term)) (up_Term_Term sigma) x =
-  up_Term_Term theta x.
+  funcomp (ren_Tm (upRen_Tm_Tm zeta_Tm)) (up_Tm_Tm sigma) x =
+  up_Tm_Tm theta x.
 Proof.
 exact (fun n =>
        match n with
        | S n' =>
            eq_trans
-             (compRenRen_Term shift (upRen_Term_Term zeta_Term)
-                (funcomp shift zeta_Term) (fun x => eq_refl) (sigma n'))
+             (compRenRen_Tm shift (upRen_Tm_Tm zeta_Tm)
+                (funcomp shift zeta_Tm) (fun x => eq_refl) (sigma n'))
              (eq_trans
                 (eq_sym
-                   (compRenRen_Term zeta_Term shift (funcomp shift zeta_Term)
+                   (compRenRen_Tm zeta_Tm shift (funcomp shift zeta_Tm)
                       (fun x => eq_refl) (sigma n')))
-                (ap (ren_Term shift) (Eq n')))
+                (ap (ren_Tm shift) (Eq n')))
        | O => eq_refl
        end).
 Qed.
 
-Fixpoint compSubstRen_Term (sigma_Term : nat -> Term)
-(zeta_Term : nat -> nat) (theta_Term : nat -> Term)
-(Eq_Term : forall x, funcomp (ren_Term zeta_Term) sigma_Term x = theta_Term x)
-(s : Term) {struct s} :
-ren_Term zeta_Term (subst_Term sigma_Term s) = subst_Term theta_Term s :=
+Fixpoint compSubstRen_Tm (sigma_Tm : nat -> Tm) (zeta_Tm : nat -> nat)
+(theta_Tm : nat -> Tm)
+(Eq_Tm : forall x, funcomp (ren_Tm zeta_Tm) sigma_Tm x = theta_Tm x) 
+(s : Tm) {struct s} :
+ren_Tm zeta_Tm (subst_Tm sigma_Tm s) = subst_Tm theta_Tm s :=
   match s with
-  | VarTm s0 => Eq_Term s0
-  | ISort s0 => congr_ISort (eq_refl s0)
-  | Abs s0 s1 =>
-      congr_Abs
-        (compSubstRen_Term sigma_Term zeta_Term theta_Term Eq_Term s0)
-        (compSubstRen_Term (up_Term_Term sigma_Term)
-           (upRen_Term_Term zeta_Term) (up_Term_Term theta_Term)
-           (up_subst_ren_Term_Term _ _ _ Eq_Term) s1)
-  | App s0 s1 =>
-      congr_App
-        (compSubstRen_Term sigma_Term zeta_Term theta_Term Eq_Term s0)
-        (compSubstRen_Term sigma_Term zeta_Term theta_Term Eq_Term s1)
-  | Pi s0 s1 =>
-      congr_Pi (compSubstRen_Term sigma_Term zeta_Term theta_Term Eq_Term s0)
-        (compSubstRen_Term (up_Term_Term sigma_Term)
-           (upRen_Term_Term zeta_Term) (up_Term_Term theta_Term)
-           (up_subst_ren_Term_Term _ _ _ Eq_Term) s1)
+  | VarTm s0 => Eq_Tm s0
+  | TmAbs s0 =>
+      congr_TmAbs
+        (compSubstRen_Tm (up_Tm_Tm sigma_Tm) (upRen_Tm_Tm zeta_Tm)
+           (up_Tm_Tm theta_Tm) (up_subst_ren_Tm_Tm _ _ _ Eq_Tm) s0)
+  | TmApp s0 s1 =>
+      congr_TmApp (compSubstRen_Tm sigma_Tm zeta_Tm theta_Tm Eq_Tm s0)
+        (compSubstRen_Tm sigma_Tm zeta_Tm theta_Tm Eq_Tm s1)
   end.
 
-Lemma up_subst_subst_Term_Term (sigma : nat -> Term) (tau_Term : nat -> Term)
-  (theta : nat -> Term)
-  (Eq : forall x, funcomp (subst_Term tau_Term) sigma x = theta x) :
+Lemma up_subst_subst_Tm_Tm (sigma : nat -> Tm) (tau_Tm : nat -> Tm)
+  (theta : nat -> Tm)
+  (Eq : forall x, funcomp (subst_Tm tau_Tm) sigma x = theta x) :
   forall x,
-  funcomp (subst_Term (up_Term_Term tau_Term)) (up_Term_Term sigma) x =
-  up_Term_Term theta x.
+  funcomp (subst_Tm (up_Tm_Tm tau_Tm)) (up_Tm_Tm sigma) x = up_Tm_Tm theta x.
 Proof.
 exact (fun n =>
        match n with
        | S n' =>
            eq_trans
-             (compRenSubst_Term shift (up_Term_Term tau_Term)
-                (funcomp (up_Term_Term tau_Term) shift) (fun x => eq_refl)
+             (compRenSubst_Tm shift (up_Tm_Tm tau_Tm)
+                (funcomp (up_Tm_Tm tau_Tm) shift) (fun x => eq_refl)
                 (sigma n'))
              (eq_trans
                 (eq_sym
-                   (compSubstRen_Term tau_Term shift
-                      (funcomp (ren_Term shift) tau_Term) (fun x => eq_refl)
-                      (sigma n'))) (ap (ren_Term shift) (Eq n')))
+                   (compSubstRen_Tm tau_Tm shift
+                      (funcomp (ren_Tm shift) tau_Tm) (fun x => eq_refl)
+                      (sigma n'))) (ap (ren_Tm shift) (Eq n')))
        | O => eq_refl
        end).
 Qed.
 
-Fixpoint compSubstSubst_Term (sigma_Term : nat -> Term)
-(tau_Term : nat -> Term) (theta_Term : nat -> Term)
-(Eq_Term : forall x,
-           funcomp (subst_Term tau_Term) sigma_Term x = theta_Term x)
-(s : Term) {struct s} :
-subst_Term tau_Term (subst_Term sigma_Term s) = subst_Term theta_Term s :=
+Fixpoint compSubstSubst_Tm (sigma_Tm : nat -> Tm) (tau_Tm : nat -> Tm)
+(theta_Tm : nat -> Tm)
+(Eq_Tm : forall x, funcomp (subst_Tm tau_Tm) sigma_Tm x = theta_Tm x)
+(s : Tm) {struct s} :
+subst_Tm tau_Tm (subst_Tm sigma_Tm s) = subst_Tm theta_Tm s :=
   match s with
-  | VarTm s0 => Eq_Term s0
-  | ISort s0 => congr_ISort (eq_refl s0)
-  | Abs s0 s1 =>
-      congr_Abs
-        (compSubstSubst_Term sigma_Term tau_Term theta_Term Eq_Term s0)
-        (compSubstSubst_Term (up_Term_Term sigma_Term)
-           (up_Term_Term tau_Term) (up_Term_Term theta_Term)
-           (up_subst_subst_Term_Term _ _ _ Eq_Term) s1)
-  | App s0 s1 =>
-      congr_App
-        (compSubstSubst_Term sigma_Term tau_Term theta_Term Eq_Term s0)
-        (compSubstSubst_Term sigma_Term tau_Term theta_Term Eq_Term s1)
-  | Pi s0 s1 =>
-      congr_Pi
-        (compSubstSubst_Term sigma_Term tau_Term theta_Term Eq_Term s0)
-        (compSubstSubst_Term (up_Term_Term sigma_Term)
-           (up_Term_Term tau_Term) (up_Term_Term theta_Term)
-           (up_subst_subst_Term_Term _ _ _ Eq_Term) s1)
+  | VarTm s0 => Eq_Tm s0
+  | TmAbs s0 =>
+      congr_TmAbs
+        (compSubstSubst_Tm (up_Tm_Tm sigma_Tm) (up_Tm_Tm tau_Tm)
+           (up_Tm_Tm theta_Tm) (up_subst_subst_Tm_Tm _ _ _ Eq_Tm) s0)
+  | TmApp s0 s1 =>
+      congr_TmApp (compSubstSubst_Tm sigma_Tm tau_Tm theta_Tm Eq_Tm s0)
+        (compSubstSubst_Tm sigma_Tm tau_Tm theta_Tm Eq_Tm s1)
   end.
 
-Lemma renRen_Term (xi_Term : nat -> nat) (zeta_Term : nat -> nat) (s : Term)
-  :
-  ren_Term zeta_Term (ren_Term xi_Term s) =
-  ren_Term (funcomp zeta_Term xi_Term) s.
+Lemma renRen_Tm (xi_Tm : nat -> nat) (zeta_Tm : nat -> nat) (s : Tm) :
+  ren_Tm zeta_Tm (ren_Tm xi_Tm s) = ren_Tm (funcomp zeta_Tm xi_Tm) s.
 Proof.
-exact (compRenRen_Term xi_Term zeta_Term _ (fun n => eq_refl) s).
+exact (compRenRen_Tm xi_Tm zeta_Tm _ (fun n => eq_refl) s).
 Qed.
 
-Lemma renRen'_Term_pointwise (xi_Term : nat -> nat) (zeta_Term : nat -> nat)
-  :
-  pointwise_relation _ eq (funcomp (ren_Term zeta_Term) (ren_Term xi_Term))
-    (ren_Term (funcomp zeta_Term xi_Term)).
+Lemma renRen'_Tm_pointwise (xi_Tm : nat -> nat) (zeta_Tm : nat -> nat) :
+  pointwise_relation _ eq (funcomp (ren_Tm zeta_Tm) (ren_Tm xi_Tm))
+    (ren_Tm (funcomp zeta_Tm xi_Tm)).
 Proof.
-exact (fun s => compRenRen_Term xi_Term zeta_Term _ (fun n => eq_refl) s).
+exact (fun s => compRenRen_Tm xi_Tm zeta_Tm _ (fun n => eq_refl) s).
 Qed.
 
-Lemma renSubst_Term (xi_Term : nat -> nat) (tau_Term : nat -> Term)
-  (s : Term) :
-  subst_Term tau_Term (ren_Term xi_Term s) =
-  subst_Term (funcomp tau_Term xi_Term) s.
+Lemma renSubst_Tm (xi_Tm : nat -> nat) (tau_Tm : nat -> Tm) (s : Tm) :
+  subst_Tm tau_Tm (ren_Tm xi_Tm s) = subst_Tm (funcomp tau_Tm xi_Tm) s.
 Proof.
-exact (compRenSubst_Term xi_Term tau_Term _ (fun n => eq_refl) s).
+exact (compRenSubst_Tm xi_Tm tau_Tm _ (fun n => eq_refl) s).
 Qed.
 
-Lemma renSubst_Term_pointwise (xi_Term : nat -> nat) (tau_Term : nat -> Term)
-  :
-  pointwise_relation _ eq (funcomp (subst_Term tau_Term) (ren_Term xi_Term))
-    (subst_Term (funcomp tau_Term xi_Term)).
+Lemma renSubst_Tm_pointwise (xi_Tm : nat -> nat) (tau_Tm : nat -> Tm) :
+  pointwise_relation _ eq (funcomp (subst_Tm tau_Tm) (ren_Tm xi_Tm))
+    (subst_Tm (funcomp tau_Tm xi_Tm)).
 Proof.
-exact (fun s => compRenSubst_Term xi_Term tau_Term _ (fun n => eq_refl) s).
+exact (fun s => compRenSubst_Tm xi_Tm tau_Tm _ (fun n => eq_refl) s).
 Qed.
 
-Lemma substRen_Term (sigma_Term : nat -> Term) (zeta_Term : nat -> nat)
-  (s : Term) :
-  ren_Term zeta_Term (subst_Term sigma_Term s) =
-  subst_Term (funcomp (ren_Term zeta_Term) sigma_Term) s.
+Lemma substRen_Tm (sigma_Tm : nat -> Tm) (zeta_Tm : nat -> nat) (s : Tm) :
+  ren_Tm zeta_Tm (subst_Tm sigma_Tm s) =
+  subst_Tm (funcomp (ren_Tm zeta_Tm) sigma_Tm) s.
 Proof.
-exact (compSubstRen_Term sigma_Term zeta_Term _ (fun n => eq_refl) s).
+exact (compSubstRen_Tm sigma_Tm zeta_Tm _ (fun n => eq_refl) s).
 Qed.
 
-Lemma substRen_Term_pointwise (sigma_Term : nat -> Term)
-  (zeta_Term : nat -> nat) :
-  pointwise_relation _ eq
-    (funcomp (ren_Term zeta_Term) (subst_Term sigma_Term))
-    (subst_Term (funcomp (ren_Term zeta_Term) sigma_Term)).
+Lemma substRen_Tm_pointwise (sigma_Tm : nat -> Tm) (zeta_Tm : nat -> nat) :
+  pointwise_relation _ eq (funcomp (ren_Tm zeta_Tm) (subst_Tm sigma_Tm))
+    (subst_Tm (funcomp (ren_Tm zeta_Tm) sigma_Tm)).
 Proof.
-exact (fun s => compSubstRen_Term sigma_Term zeta_Term _ (fun n => eq_refl) s).
+exact (fun s => compSubstRen_Tm sigma_Tm zeta_Tm _ (fun n => eq_refl) s).
 Qed.
 
-Lemma substSubst_Term (sigma_Term : nat -> Term) (tau_Term : nat -> Term)
-  (s : Term) :
-  subst_Term tau_Term (subst_Term sigma_Term s) =
-  subst_Term (funcomp (subst_Term tau_Term) sigma_Term) s.
+Lemma substSubst_Tm (sigma_Tm : nat -> Tm) (tau_Tm : nat -> Tm) (s : Tm) :
+  subst_Tm tau_Tm (subst_Tm sigma_Tm s) =
+  subst_Tm (funcomp (subst_Tm tau_Tm) sigma_Tm) s.
 Proof.
-exact (compSubstSubst_Term sigma_Term tau_Term _ (fun n => eq_refl) s).
+exact (compSubstSubst_Tm sigma_Tm tau_Tm _ (fun n => eq_refl) s).
 Qed.
 
-Lemma substSubst_Term_pointwise (sigma_Term : nat -> Term)
-  (tau_Term : nat -> Term) :
-  pointwise_relation _ eq
-    (funcomp (subst_Term tau_Term) (subst_Term sigma_Term))
-    (subst_Term (funcomp (subst_Term tau_Term) sigma_Term)).
+Lemma substSubst_Tm_pointwise (sigma_Tm : nat -> Tm) (tau_Tm : nat -> Tm) :
+  pointwise_relation _ eq (funcomp (subst_Tm tau_Tm) (subst_Tm sigma_Tm))
+    (subst_Tm (funcomp (subst_Tm tau_Tm) sigma_Tm)).
 Proof.
-exact (fun s =>
-       compSubstSubst_Term sigma_Term tau_Term _ (fun n => eq_refl) s).
+exact (fun s => compSubstSubst_Tm sigma_Tm tau_Tm _ (fun n => eq_refl) s).
 Qed.
 
-Lemma rinstInst_up_Term_Term (xi : nat -> nat) (sigma : nat -> Term)
+Lemma rinstInst_up_Tm_Tm (xi : nat -> nat) (sigma : nat -> Tm)
   (Eq : forall x, funcomp (VarTm) xi x = sigma x) :
-  forall x, funcomp (VarTm) (upRen_Term_Term xi) x = up_Term_Term sigma x.
+  forall x, funcomp (VarTm) (upRen_Tm_Tm xi) x = up_Tm_Tm sigma x.
 Proof.
 exact (fun n =>
        match n with
-       | S n' => ap (ren_Term shift) (Eq n')
+       | S n' => ap (ren_Tm shift) (Eq n')
        | O => eq_refl
        end).
 Qed.
 
-Fixpoint rinst_inst_Term (xi_Term : nat -> nat) (sigma_Term : nat -> Term)
-(Eq_Term : forall x, funcomp (VarTm) xi_Term x = sigma_Term x) (s : Term)
-{struct s} : ren_Term xi_Term s = subst_Term sigma_Term s :=
+Fixpoint rinst_inst_Tm (xi_Tm : nat -> nat) (sigma_Tm : nat -> Tm)
+(Eq_Tm : forall x, funcomp (VarTm) xi_Tm x = sigma_Tm x) (s : Tm) {struct s}
+   : ren_Tm xi_Tm s = subst_Tm sigma_Tm s :=
   match s with
-  | VarTm s0 => Eq_Term s0
-  | ISort s0 => congr_ISort (eq_refl s0)
-  | Abs s0 s1 =>
-      congr_Abs (rinst_inst_Term xi_Term sigma_Term Eq_Term s0)
-        (rinst_inst_Term (upRen_Term_Term xi_Term) (up_Term_Term sigma_Term)
-           (rinstInst_up_Term_Term _ _ Eq_Term) s1)
-  | App s0 s1 =>
-      congr_App (rinst_inst_Term xi_Term sigma_Term Eq_Term s0)
-        (rinst_inst_Term xi_Term sigma_Term Eq_Term s1)
-  | Pi s0 s1 =>
-      congr_Pi (rinst_inst_Term xi_Term sigma_Term Eq_Term s0)
-        (rinst_inst_Term (upRen_Term_Term xi_Term) (up_Term_Term sigma_Term)
-           (rinstInst_up_Term_Term _ _ Eq_Term) s1)
+  | VarTm s0 => Eq_Tm s0
+  | TmAbs s0 =>
+      congr_TmAbs
+        (rinst_inst_Tm (upRen_Tm_Tm xi_Tm) (up_Tm_Tm sigma_Tm)
+           (rinstInst_up_Tm_Tm _ _ Eq_Tm) s0)
+  | TmApp s0 s1 =>
+      congr_TmApp (rinst_inst_Tm xi_Tm sigma_Tm Eq_Tm s0)
+        (rinst_inst_Tm xi_Tm sigma_Tm Eq_Tm s1)
   end.
 
-Lemma rinstInst'_Term (xi_Term : nat -> nat) (s : Term) :
-  ren_Term xi_Term s = subst_Term (funcomp (VarTm) xi_Term) s.
+Lemma rinstInst'_Tm (xi_Tm : nat -> nat) (s : Tm) :
+  ren_Tm xi_Tm s = subst_Tm (funcomp (VarTm) xi_Tm) s.
 Proof.
-exact (rinst_inst_Term xi_Term _ (fun n => eq_refl) s).
+exact (rinst_inst_Tm xi_Tm _ (fun n => eq_refl) s).
 Qed.
 
-Lemma rinstInst'_Term_pointwise (xi_Term : nat -> nat) :
-  pointwise_relation _ eq (ren_Term xi_Term)
-    (subst_Term (funcomp (VarTm) xi_Term)).
+Lemma rinstInst'_Tm_pointwise (xi_Tm : nat -> nat) :
+  pointwise_relation _ eq (ren_Tm xi_Tm) (subst_Tm (funcomp (VarTm) xi_Tm)).
 Proof.
-exact (fun s => rinst_inst_Term xi_Term _ (fun n => eq_refl) s).
+exact (fun s => rinst_inst_Tm xi_Tm _ (fun n => eq_refl) s).
 Qed.
 
-Lemma instId'_Term (s : Term) : subst_Term (VarTm) s = s.
+Lemma instId'_Tm (s : Tm) : subst_Tm (VarTm) s = s.
 Proof.
-exact (idSubst_Term (VarTm) (fun n => eq_refl) s).
+exact (idSubst_Tm (VarTm) (fun n => eq_refl) s).
 Qed.
 
-Lemma instId'_Term_pointwise :
-  pointwise_relation _ eq (subst_Term (VarTm)) id.
+Lemma instId'_Tm_pointwise : pointwise_relation _ eq (subst_Tm (VarTm)) id.
 Proof.
-exact (fun s => idSubst_Term (VarTm) (fun n => eq_refl) s).
+exact (fun s => idSubst_Tm (VarTm) (fun n => eq_refl) s).
 Qed.
 
-Lemma rinstId'_Term (s : Term) : ren_Term id s = s.
+Lemma rinstId'_Tm (s : Tm) : ren_Tm id s = s.
 Proof.
-exact (eq_ind_r (fun t => t = s) (instId'_Term s) (rinstInst'_Term id s)).
+exact (eq_ind_r (fun t => t = s) (instId'_Tm s) (rinstInst'_Tm id s)).
 Qed.
 
-Lemma rinstId'_Term_pointwise : pointwise_relation _ eq (@ren_Term id) id.
+Lemma rinstId'_Tm_pointwise : pointwise_relation _ eq (@ren_Tm id) id.
 Proof.
-exact (fun s =>
-       eq_ind_r (fun t => t = s) (instId'_Term s) (rinstInst'_Term id s)).
+exact (fun s => eq_ind_r (fun t => t = s) (instId'_Tm s) (rinstInst'_Tm id s)).
 Qed.
 
-Lemma varL'_Term (sigma_Term : nat -> Term) (x : nat) :
-  subst_Term sigma_Term (VarTm x) = sigma_Term x.
+Lemma varL'_Tm (sigma_Tm : nat -> Tm) (x : nat) :
+  subst_Tm sigma_Tm (VarTm x) = sigma_Tm x.
 Proof.
 exact (eq_refl).
 Qed.
 
-Lemma varL'_Term_pointwise (sigma_Term : nat -> Term) :
-  pointwise_relation _ eq (funcomp (subst_Term sigma_Term) (VarTm))
-    sigma_Term.
+Lemma varL'_Tm_pointwise (sigma_Tm : nat -> Tm) :
+  pointwise_relation _ eq (funcomp (subst_Tm sigma_Tm) (VarTm)) sigma_Tm.
 Proof.
 exact (fun x => eq_refl).
 Qed.
 
-Lemma varLRen'_Term (xi_Term : nat -> nat) (x : nat) :
-  ren_Term xi_Term (VarTm x) = VarTm (xi_Term x).
+Lemma varLRen'_Tm (xi_Tm : nat -> nat) (x : nat) :
+  ren_Tm xi_Tm (VarTm x) = VarTm (xi_Tm x).
 Proof.
 exact (eq_refl).
 Qed.
 
-Lemma varLRen'_Term_pointwise (xi_Term : nat -> nat) :
-  pointwise_relation _ eq (funcomp (ren_Term xi_Term) (VarTm))
-    (funcomp (VarTm) xi_Term).
+Lemma varLRen'_Tm_pointwise (xi_Tm : nat -> nat) :
+  pointwise_relation _ eq (funcomp (ren_Tm xi_Tm) (VarTm))
+    (funcomp (VarTm) xi_Tm).
 Proof.
 exact (fun x => eq_refl).
 Qed.
 
-Class Up_Term X Y :=
-    up_Term : X -> Y.
+Inductive Ty : Type :=
+  | VarTy : nat -> Ty
+  | TyAbs : Ty -> Ty
+  | TyApp : Ty -> Ty -> Ty.
 
-#[global]Instance Subst_Term : (Subst1 _ _ _) := @subst_Term.
+Lemma congr_TyAbs {s0 : Ty} {t0 : Ty} (H0 : s0 = t0) : TyAbs s0 = TyAbs t0.
+Proof.
+exact (eq_trans eq_refl (ap (fun x => TyAbs x) H0)).
+Qed.
 
-#[global]Instance Up_Term_Term : (Up_Term _ _) := @up_Term_Term.
+Lemma congr_TyApp {s0 : Ty} {s1 : Ty} {t0 : Ty} {t1 : Ty} (H0 : s0 = t0)
+  (H1 : s1 = t1) : TyApp s0 s1 = TyApp t0 t1.
+Proof.
+exact (eq_trans (eq_trans eq_refl (ap (fun x => TyApp x s1) H0))
+         (ap (fun x => TyApp t0 x) H1)).
+Qed.
 
-#[global]Instance Ren_Term : (Ren1 _ _ _) := @ren_Term.
+Lemma upRen_Ty_Ty (xi : nat -> nat) : nat -> nat.
+Proof.
+exact (up_ren xi).
+Defined.
+
+Fixpoint ren_Ty (xi_Ty : nat -> nat) (s : Ty) {struct s} : Ty :=
+  match s with
+  | VarTy s0 => VarTy (xi_Ty s0)
+  | TyAbs s0 => TyAbs (ren_Ty (upRen_Ty_Ty xi_Ty) s0)
+  | TyApp s0 s1 => TyApp (ren_Ty xi_Ty s0) (ren_Ty xi_Ty s1)
+  end.
+
+Lemma up_Ty_Ty (sigma : nat -> Ty) : nat -> Ty.
+Proof.
+exact (scons (VarTy var_zero) (funcomp (ren_Ty shift) sigma)).
+Defined.
+
+Fixpoint subst_Ty (sigma_Ty : nat -> Ty) (s : Ty) {struct s} : Ty :=
+  match s with
+  | VarTy s0 => sigma_Ty s0
+  | TyAbs s0 => TyAbs (subst_Ty (up_Ty_Ty sigma_Ty) s0)
+  | TyApp s0 s1 => TyApp (subst_Ty sigma_Ty s0) (subst_Ty sigma_Ty s1)
+  end.
+
+Lemma upId_Ty_Ty (sigma : nat -> Ty) (Eq : forall x, sigma x = VarTy x) :
+  forall x, up_Ty_Ty sigma x = VarTy x.
+Proof.
+exact (fun n =>
+       match n with
+       | S n' => ap (ren_Ty shift) (Eq n')
+       | O => eq_refl
+       end).
+Qed.
+
+Fixpoint idSubst_Ty (sigma_Ty : nat -> Ty)
+(Eq_Ty : forall x, sigma_Ty x = VarTy x) (s : Ty) {struct s} :
+subst_Ty sigma_Ty s = s :=
+  match s with
+  | VarTy s0 => Eq_Ty s0
+  | TyAbs s0 =>
+      congr_TyAbs (idSubst_Ty (up_Ty_Ty sigma_Ty) (upId_Ty_Ty _ Eq_Ty) s0)
+  | TyApp s0 s1 =>
+      congr_TyApp (idSubst_Ty sigma_Ty Eq_Ty s0)
+        (idSubst_Ty sigma_Ty Eq_Ty s1)
+  end.
+
+Lemma upExtRen_Ty_Ty (xi : nat -> nat) (zeta : nat -> nat)
+  (Eq : forall x, xi x = zeta x) :
+  forall x, upRen_Ty_Ty xi x = upRen_Ty_Ty zeta x.
+Proof.
+exact (fun n => match n with
+                | S n' => ap shift (Eq n')
+                | O => eq_refl
+                end).
+Qed.
+
+Fixpoint extRen_Ty (xi_Ty : nat -> nat) (zeta_Ty : nat -> nat)
+(Eq_Ty : forall x, xi_Ty x = zeta_Ty x) (s : Ty) {struct s} :
+ren_Ty xi_Ty s = ren_Ty zeta_Ty s :=
+  match s with
+  | VarTy s0 => ap (VarTy) (Eq_Ty s0)
+  | TyAbs s0 =>
+      congr_TyAbs
+        (extRen_Ty (upRen_Ty_Ty xi_Ty) (upRen_Ty_Ty zeta_Ty)
+           (upExtRen_Ty_Ty _ _ Eq_Ty) s0)
+  | TyApp s0 s1 =>
+      congr_TyApp (extRen_Ty xi_Ty zeta_Ty Eq_Ty s0)
+        (extRen_Ty xi_Ty zeta_Ty Eq_Ty s1)
+  end.
+
+Lemma upExt_Ty_Ty (sigma : nat -> Ty) (tau : nat -> Ty)
+  (Eq : forall x, sigma x = tau x) :
+  forall x, up_Ty_Ty sigma x = up_Ty_Ty tau x.
+Proof.
+exact (fun n =>
+       match n with
+       | S n' => ap (ren_Ty shift) (Eq n')
+       | O => eq_refl
+       end).
+Qed.
+
+Fixpoint ext_Ty (sigma_Ty : nat -> Ty) (tau_Ty : nat -> Ty)
+(Eq_Ty : forall x, sigma_Ty x = tau_Ty x) (s : Ty) {struct s} :
+subst_Ty sigma_Ty s = subst_Ty tau_Ty s :=
+  match s with
+  | VarTy s0 => Eq_Ty s0
+  | TyAbs s0 =>
+      congr_TyAbs
+        (ext_Ty (up_Ty_Ty sigma_Ty) (up_Ty_Ty tau_Ty) (upExt_Ty_Ty _ _ Eq_Ty)
+           s0)
+  | TyApp s0 s1 =>
+      congr_TyApp (ext_Ty sigma_Ty tau_Ty Eq_Ty s0)
+        (ext_Ty sigma_Ty tau_Ty Eq_Ty s1)
+  end.
+
+Lemma up_ren_ren_Ty_Ty (xi : nat -> nat) (zeta : nat -> nat)
+  (rho : nat -> nat) (Eq : forall x, funcomp zeta xi x = rho x) :
+  forall x, funcomp (upRen_Ty_Ty zeta) (upRen_Ty_Ty xi) x = upRen_Ty_Ty rho x.
+Proof.
+exact (up_ren_ren xi zeta rho Eq).
+Qed.
+
+Fixpoint compRenRen_Ty (xi_Ty : nat -> nat) (zeta_Ty : nat -> nat)
+(rho_Ty : nat -> nat) (Eq_Ty : forall x, funcomp zeta_Ty xi_Ty x = rho_Ty x)
+(s : Ty) {struct s} : ren_Ty zeta_Ty (ren_Ty xi_Ty s) = ren_Ty rho_Ty s :=
+  match s with
+  | VarTy s0 => ap (VarTy) (Eq_Ty s0)
+  | TyAbs s0 =>
+      congr_TyAbs
+        (compRenRen_Ty (upRen_Ty_Ty xi_Ty) (upRen_Ty_Ty zeta_Ty)
+           (upRen_Ty_Ty rho_Ty) (up_ren_ren _ _ _ Eq_Ty) s0)
+  | TyApp s0 s1 =>
+      congr_TyApp (compRenRen_Ty xi_Ty zeta_Ty rho_Ty Eq_Ty s0)
+        (compRenRen_Ty xi_Ty zeta_Ty rho_Ty Eq_Ty s1)
+  end.
+
+Lemma up_ren_subst_Ty_Ty (xi : nat -> nat) (tau : nat -> Ty)
+  (theta : nat -> Ty) (Eq : forall x, funcomp tau xi x = theta x) :
+  forall x, funcomp (up_Ty_Ty tau) (upRen_Ty_Ty xi) x = up_Ty_Ty theta x.
+Proof.
+exact (fun n =>
+       match n with
+       | S n' => ap (ren_Ty shift) (Eq n')
+       | O => eq_refl
+       end).
+Qed.
+
+Fixpoint compRenSubst_Ty (xi_Ty : nat -> nat) (tau_Ty : nat -> Ty)
+(theta_Ty : nat -> Ty)
+(Eq_Ty : forall x, funcomp tau_Ty xi_Ty x = theta_Ty x) (s : Ty) {struct s} :
+subst_Ty tau_Ty (ren_Ty xi_Ty s) = subst_Ty theta_Ty s :=
+  match s with
+  | VarTy s0 => Eq_Ty s0
+  | TyAbs s0 =>
+      congr_TyAbs
+        (compRenSubst_Ty (upRen_Ty_Ty xi_Ty) (up_Ty_Ty tau_Ty)
+           (up_Ty_Ty theta_Ty) (up_ren_subst_Ty_Ty _ _ _ Eq_Ty) s0)
+  | TyApp s0 s1 =>
+      congr_TyApp (compRenSubst_Ty xi_Ty tau_Ty theta_Ty Eq_Ty s0)
+        (compRenSubst_Ty xi_Ty tau_Ty theta_Ty Eq_Ty s1)
+  end.
+
+Lemma up_subst_ren_Ty_Ty (sigma : nat -> Ty) (zeta_Ty : nat -> nat)
+  (theta : nat -> Ty)
+  (Eq : forall x, funcomp (ren_Ty zeta_Ty) sigma x = theta x) :
+  forall x,
+  funcomp (ren_Ty (upRen_Ty_Ty zeta_Ty)) (up_Ty_Ty sigma) x =
+  up_Ty_Ty theta x.
+Proof.
+exact (fun n =>
+       match n with
+       | S n' =>
+           eq_trans
+             (compRenRen_Ty shift (upRen_Ty_Ty zeta_Ty)
+                (funcomp shift zeta_Ty) (fun x => eq_refl) (sigma n'))
+             (eq_trans
+                (eq_sym
+                   (compRenRen_Ty zeta_Ty shift (funcomp shift zeta_Ty)
+                      (fun x => eq_refl) (sigma n')))
+                (ap (ren_Ty shift) (Eq n')))
+       | O => eq_refl
+       end).
+Qed.
+
+Fixpoint compSubstRen_Ty (sigma_Ty : nat -> Ty) (zeta_Ty : nat -> nat)
+(theta_Ty : nat -> Ty)
+(Eq_Ty : forall x, funcomp (ren_Ty zeta_Ty) sigma_Ty x = theta_Ty x) 
+(s : Ty) {struct s} :
+ren_Ty zeta_Ty (subst_Ty sigma_Ty s) = subst_Ty theta_Ty s :=
+  match s with
+  | VarTy s0 => Eq_Ty s0
+  | TyAbs s0 =>
+      congr_TyAbs
+        (compSubstRen_Ty (up_Ty_Ty sigma_Ty) (upRen_Ty_Ty zeta_Ty)
+           (up_Ty_Ty theta_Ty) (up_subst_ren_Ty_Ty _ _ _ Eq_Ty) s0)
+  | TyApp s0 s1 =>
+      congr_TyApp (compSubstRen_Ty sigma_Ty zeta_Ty theta_Ty Eq_Ty s0)
+        (compSubstRen_Ty sigma_Ty zeta_Ty theta_Ty Eq_Ty s1)
+  end.
+
+Lemma up_subst_subst_Ty_Ty (sigma : nat -> Ty) (tau_Ty : nat -> Ty)
+  (theta : nat -> Ty)
+  (Eq : forall x, funcomp (subst_Ty tau_Ty) sigma x = theta x) :
+  forall x,
+  funcomp (subst_Ty (up_Ty_Ty tau_Ty)) (up_Ty_Ty sigma) x = up_Ty_Ty theta x.
+Proof.
+exact (fun n =>
+       match n with
+       | S n' =>
+           eq_trans
+             (compRenSubst_Ty shift (up_Ty_Ty tau_Ty)
+                (funcomp (up_Ty_Ty tau_Ty) shift) (fun x => eq_refl)
+                (sigma n'))
+             (eq_trans
+                (eq_sym
+                   (compSubstRen_Ty tau_Ty shift
+                      (funcomp (ren_Ty shift) tau_Ty) (fun x => eq_refl)
+                      (sigma n'))) (ap (ren_Ty shift) (Eq n')))
+       | O => eq_refl
+       end).
+Qed.
+
+Fixpoint compSubstSubst_Ty (sigma_Ty : nat -> Ty) (tau_Ty : nat -> Ty)
+(theta_Ty : nat -> Ty)
+(Eq_Ty : forall x, funcomp (subst_Ty tau_Ty) sigma_Ty x = theta_Ty x)
+(s : Ty) {struct s} :
+subst_Ty tau_Ty (subst_Ty sigma_Ty s) = subst_Ty theta_Ty s :=
+  match s with
+  | VarTy s0 => Eq_Ty s0
+  | TyAbs s0 =>
+      congr_TyAbs
+        (compSubstSubst_Ty (up_Ty_Ty sigma_Ty) (up_Ty_Ty tau_Ty)
+           (up_Ty_Ty theta_Ty) (up_subst_subst_Ty_Ty _ _ _ Eq_Ty) s0)
+  | TyApp s0 s1 =>
+      congr_TyApp (compSubstSubst_Ty sigma_Ty tau_Ty theta_Ty Eq_Ty s0)
+        (compSubstSubst_Ty sigma_Ty tau_Ty theta_Ty Eq_Ty s1)
+  end.
+
+Lemma renRen_Ty (xi_Ty : nat -> nat) (zeta_Ty : nat -> nat) (s : Ty) :
+  ren_Ty zeta_Ty (ren_Ty xi_Ty s) = ren_Ty (funcomp zeta_Ty xi_Ty) s.
+Proof.
+exact (compRenRen_Ty xi_Ty zeta_Ty _ (fun n => eq_refl) s).
+Qed.
+
+Lemma renRen'_Ty_pointwise (xi_Ty : nat -> nat) (zeta_Ty : nat -> nat) :
+  pointwise_relation _ eq (funcomp (ren_Ty zeta_Ty) (ren_Ty xi_Ty))
+    (ren_Ty (funcomp zeta_Ty xi_Ty)).
+Proof.
+exact (fun s => compRenRen_Ty xi_Ty zeta_Ty _ (fun n => eq_refl) s).
+Qed.
+
+Lemma renSubst_Ty (xi_Ty : nat -> nat) (tau_Ty : nat -> Ty) (s : Ty) :
+  subst_Ty tau_Ty (ren_Ty xi_Ty s) = subst_Ty (funcomp tau_Ty xi_Ty) s.
+Proof.
+exact (compRenSubst_Ty xi_Ty tau_Ty _ (fun n => eq_refl) s).
+Qed.
+
+Lemma renSubst_Ty_pointwise (xi_Ty : nat -> nat) (tau_Ty : nat -> Ty) :
+  pointwise_relation _ eq (funcomp (subst_Ty tau_Ty) (ren_Ty xi_Ty))
+    (subst_Ty (funcomp tau_Ty xi_Ty)).
+Proof.
+exact (fun s => compRenSubst_Ty xi_Ty tau_Ty _ (fun n => eq_refl) s).
+Qed.
+
+Lemma substRen_Ty (sigma_Ty : nat -> Ty) (zeta_Ty : nat -> nat) (s : Ty) :
+  ren_Ty zeta_Ty (subst_Ty sigma_Ty s) =
+  subst_Ty (funcomp (ren_Ty zeta_Ty) sigma_Ty) s.
+Proof.
+exact (compSubstRen_Ty sigma_Ty zeta_Ty _ (fun n => eq_refl) s).
+Qed.
+
+Lemma substRen_Ty_pointwise (sigma_Ty : nat -> Ty) (zeta_Ty : nat -> nat) :
+  pointwise_relation _ eq (funcomp (ren_Ty zeta_Ty) (subst_Ty sigma_Ty))
+    (subst_Ty (funcomp (ren_Ty zeta_Ty) sigma_Ty)).
+Proof.
+exact (fun s => compSubstRen_Ty sigma_Ty zeta_Ty _ (fun n => eq_refl) s).
+Qed.
+
+Lemma substSubst_Ty (sigma_Ty : nat -> Ty) (tau_Ty : nat -> Ty) (s : Ty) :
+  subst_Ty tau_Ty (subst_Ty sigma_Ty s) =
+  subst_Ty (funcomp (subst_Ty tau_Ty) sigma_Ty) s.
+Proof.
+exact (compSubstSubst_Ty sigma_Ty tau_Ty _ (fun n => eq_refl) s).
+Qed.
+
+Lemma substSubst_Ty_pointwise (sigma_Ty : nat -> Ty) (tau_Ty : nat -> Ty) :
+  pointwise_relation _ eq (funcomp (subst_Ty tau_Ty) (subst_Ty sigma_Ty))
+    (subst_Ty (funcomp (subst_Ty tau_Ty) sigma_Ty)).
+Proof.
+exact (fun s => compSubstSubst_Ty sigma_Ty tau_Ty _ (fun n => eq_refl) s).
+Qed.
+
+Lemma rinstInst_up_Ty_Ty (xi : nat -> nat) (sigma : nat -> Ty)
+  (Eq : forall x, funcomp (VarTy) xi x = sigma x) :
+  forall x, funcomp (VarTy) (upRen_Ty_Ty xi) x = up_Ty_Ty sigma x.
+Proof.
+exact (fun n =>
+       match n with
+       | S n' => ap (ren_Ty shift) (Eq n')
+       | O => eq_refl
+       end).
+Qed.
+
+Fixpoint rinst_inst_Ty (xi_Ty : nat -> nat) (sigma_Ty : nat -> Ty)
+(Eq_Ty : forall x, funcomp (VarTy) xi_Ty x = sigma_Ty x) (s : Ty) {struct s}
+   : ren_Ty xi_Ty s = subst_Ty sigma_Ty s :=
+  match s with
+  | VarTy s0 => Eq_Ty s0
+  | TyAbs s0 =>
+      congr_TyAbs
+        (rinst_inst_Ty (upRen_Ty_Ty xi_Ty) (up_Ty_Ty sigma_Ty)
+           (rinstInst_up_Ty_Ty _ _ Eq_Ty) s0)
+  | TyApp s0 s1 =>
+      congr_TyApp (rinst_inst_Ty xi_Ty sigma_Ty Eq_Ty s0)
+        (rinst_inst_Ty xi_Ty sigma_Ty Eq_Ty s1)
+  end.
+
+Lemma rinstInst'_Ty (xi_Ty : nat -> nat) (s : Ty) :
+  ren_Ty xi_Ty s = subst_Ty (funcomp (VarTy) xi_Ty) s.
+Proof.
+exact (rinst_inst_Ty xi_Ty _ (fun n => eq_refl) s).
+Qed.
+
+Lemma rinstInst'_Ty_pointwise (xi_Ty : nat -> nat) :
+  pointwise_relation _ eq (ren_Ty xi_Ty) (subst_Ty (funcomp (VarTy) xi_Ty)).
+Proof.
+exact (fun s => rinst_inst_Ty xi_Ty _ (fun n => eq_refl) s).
+Qed.
+
+Lemma instId'_Ty (s : Ty) : subst_Ty (VarTy) s = s.
+Proof.
+exact (idSubst_Ty (VarTy) (fun n => eq_refl) s).
+Qed.
+
+Lemma instId'_Ty_pointwise : pointwise_relation _ eq (subst_Ty (VarTy)) id.
+Proof.
+exact (fun s => idSubst_Ty (VarTy) (fun n => eq_refl) s).
+Qed.
+
+Lemma rinstId'_Ty (s : Ty) : ren_Ty id s = s.
+Proof.
+exact (eq_ind_r (fun t => t = s) (instId'_Ty s) (rinstInst'_Ty id s)).
+Qed.
+
+Lemma rinstId'_Ty_pointwise : pointwise_relation _ eq (@ren_Ty id) id.
+Proof.
+exact (fun s => eq_ind_r (fun t => t = s) (instId'_Ty s) (rinstInst'_Ty id s)).
+Qed.
+
+Lemma varL'_Ty (sigma_Ty : nat -> Ty) (x : nat) :
+  subst_Ty sigma_Ty (VarTy x) = sigma_Ty x.
+Proof.
+exact (eq_refl).
+Qed.
+
+Lemma varL'_Ty_pointwise (sigma_Ty : nat -> Ty) :
+  pointwise_relation _ eq (funcomp (subst_Ty sigma_Ty) (VarTy)) sigma_Ty.
+Proof.
+exact (fun x => eq_refl).
+Qed.
+
+Lemma varLRen'_Ty (xi_Ty : nat -> nat) (x : nat) :
+  ren_Ty xi_Ty (VarTy x) = VarTy (xi_Ty x).
+Proof.
+exact (eq_refl).
+Qed.
+
+Lemma varLRen'_Ty_pointwise (xi_Ty : nat -> nat) :
+  pointwise_relation _ eq (funcomp (ren_Ty xi_Ty) (VarTy))
+    (funcomp (VarTy) xi_Ty).
+Proof.
+exact (fun x => eq_refl).
+Qed.
+
+Class Up_Ty X Y :=
+    up_Ty : X -> Y.
+
+Class Up_Tm X Y :=
+    up_Tm : X -> Y.
+
+#[global]Instance Subst_Ty : (Subst1 _ _ _) := @subst_Ty.
+
+#[global]Instance Up_Ty_Ty : (Up_Ty _ _) := @up_Ty_Ty.
+
+#[global]Instance Ren_Ty : (Ren1 _ _ _) := @ren_Ty.
+
+#[global]Instance VarInstance_Ty : (Var _ _) := @VarTy.
+
+#[global]Instance Subst_Tm : (Subst1 _ _ _) := @subst_Tm.
+
+#[global]Instance Up_Tm_Tm : (Up_Tm _ _) := @up_Tm_Tm.
+
+#[global]Instance Ren_Tm : (Ren1 _ _ _) := @ren_Tm.
 
 #[global]
-Instance VarInstance_Term : (Var _ _) := @VarTm.
+Instance VarInstance_Tm : (Var _ _) := @VarTm.
 
-Notation "[ sigma_Term ]" := (subst_Term sigma_Term)
+Notation "[ sigma_Ty ]" := (subst_Ty sigma_Ty)
 ( at level 1, left associativity, only printing)  : fscope.
 
-Notation "s [ sigma_Term ]" := (subst_Term sigma_Term s)
+Notation "s [ sigma_Ty ]" := (subst_Ty sigma_Ty s)
 ( at level 7, left associativity, only printing)  : subst_scope.
 
-Notation "↑__Term" := up_Term (only printing)  : subst_scope.
+Notation "↑__Ty" := up_Ty (only printing)  : subst_scope.
 
-Notation "↑__Term" := up_Term_Term (only printing)  : subst_scope.
+Notation "↑__Ty" := up_Ty_Ty (only printing)  : subst_scope.
 
-Notation "⟨ xi_Term ⟩" := (ren_Term xi_Term)
+Notation "⟨ xi_Ty ⟩" := (ren_Ty xi_Ty)
 ( at level 1, left associativity, only printing)  : fscope.
 
-Notation "s ⟨ xi_Term ⟩" := (ren_Term xi_Term s)
+Notation "s ⟨ xi_Ty ⟩" := (ren_Ty xi_Ty s)
+( at level 7, left associativity, only printing)  : subst_scope.
+
+Notation "'var'" := VarTy ( at level 1, only printing)  : subst_scope.
+
+Notation "x '__Ty'" := (@ids _ _ VarInstance_Ty x)
+( at level 5, format "x __Ty", only printing)  : subst_scope.
+
+Notation "x '__Ty'" := (VarTy x) ( at level 5, format "x __Ty")  :
+subst_scope.
+
+Notation "[ sigma_Tm ]" := (subst_Tm sigma_Tm)
+( at level 1, left associativity, only printing)  : fscope.
+
+Notation "s [ sigma_Tm ]" := (subst_Tm sigma_Tm s)
+( at level 7, left associativity, only printing)  : subst_scope.
+
+Notation "↑__Tm" := up_Tm (only printing)  : subst_scope.
+
+Notation "↑__Tm" := up_Tm_Tm (only printing)  : subst_scope.
+
+Notation "⟨ xi_Tm ⟩" := (ren_Tm xi_Tm)
+( at level 1, left associativity, only printing)  : fscope.
+
+Notation "s ⟨ xi_Tm ⟩" := (ren_Tm xi_Tm s)
 ( at level 7, left associativity, only printing)  : subst_scope.
 
 Notation "'var'" := VarTm ( at level 1, only printing)  : subst_scope.
 
-Notation "x '__Term'" := (@ids _ _ VarInstance_Term x)
-( at level 5, format "x __Term", only printing)  : subst_scope.
+Notation "x '__Tm'" := (@ids _ _ VarInstance_Tm x)
+( at level 5, format "x __Tm", only printing)  : subst_scope.
 
-Notation "x '__Term'" := (VarTm x) ( at level 5, format "x __Term")  :
+Notation "x '__Tm'" := (VarTm x) ( at level 5, format "x __Tm")  :
 subst_scope.
 
 #[global]
-Instance subst_Term_morphism :
+Instance subst_Ty_morphism :
  (Proper (respectful (pointwise_relation _ eq) (respectful eq eq))
-    (@subst_Term)).
+    (@subst_Ty)).
 Proof.
-exact (fun f_Term g_Term Eq_Term s t Eq_st =>
-       eq_ind s (fun t' => subst_Term f_Term s = subst_Term g_Term t')
-         (ext_Term f_Term g_Term Eq_Term s) t Eq_st).
+exact (fun f_Ty g_Ty Eq_Ty s t Eq_st =>
+       eq_ind s (fun t' => subst_Ty f_Ty s = subst_Ty g_Ty t')
+         (ext_Ty f_Ty g_Ty Eq_Ty s) t Eq_st).
 Qed.
 
 #[global]
-Instance subst_Term_morphism2 :
+Instance subst_Ty_morphism2 :
  (Proper (respectful (pointwise_relation _ eq) (pointwise_relation _ eq))
-    (@subst_Term)).
+    (@subst_Ty)).
 Proof.
-exact (fun f_Term g_Term Eq_Term s => ext_Term f_Term g_Term Eq_Term s).
+exact (fun f_Ty g_Ty Eq_Ty s => ext_Ty f_Ty g_Ty Eq_Ty s).
 Qed.
 
 #[global]
-Instance ren_Term_morphism :
+Instance ren_Ty_morphism :
+ (Proper (respectful (pointwise_relation _ eq) (respectful eq eq)) (@ren_Ty)).
+Proof.
+exact (fun f_Ty g_Ty Eq_Ty s t Eq_st =>
+       eq_ind s (fun t' => ren_Ty f_Ty s = ren_Ty g_Ty t')
+         (extRen_Ty f_Ty g_Ty Eq_Ty s) t Eq_st).
+Qed.
+
+#[global]
+Instance ren_Ty_morphism2 :
+ (Proper (respectful (pointwise_relation _ eq) (pointwise_relation _ eq))
+    (@ren_Ty)).
+Proof.
+exact (fun f_Ty g_Ty Eq_Ty s => extRen_Ty f_Ty g_Ty Eq_Ty s).
+Qed.
+
+#[global]
+Instance subst_Tm_morphism :
  (Proper (respectful (pointwise_relation _ eq) (respectful eq eq))
-    (@ren_Term)).
+    (@subst_Tm)).
 Proof.
-exact (fun f_Term g_Term Eq_Term s t Eq_st =>
-       eq_ind s (fun t' => ren_Term f_Term s = ren_Term g_Term t')
-         (extRen_Term f_Term g_Term Eq_Term s) t Eq_st).
+exact (fun f_Tm g_Tm Eq_Tm s t Eq_st =>
+       eq_ind s (fun t' => subst_Tm f_Tm s = subst_Tm g_Tm t')
+         (ext_Tm f_Tm g_Tm Eq_Tm s) t Eq_st).
 Qed.
 
 #[global]
-Instance ren_Term_morphism2 :
+Instance subst_Tm_morphism2 :
  (Proper (respectful (pointwise_relation _ eq) (pointwise_relation _ eq))
-    (@ren_Term)).
+    (@subst_Tm)).
 Proof.
-exact (fun f_Term g_Term Eq_Term s => extRen_Term f_Term g_Term Eq_Term s).
+exact (fun f_Tm g_Tm Eq_Tm s => ext_Tm f_Tm g_Tm Eq_Tm s).
+Qed.
+
+#[global]
+Instance ren_Tm_morphism :
+ (Proper (respectful (pointwise_relation _ eq) (respectful eq eq)) (@ren_Tm)).
+Proof.
+exact (fun f_Tm g_Tm Eq_Tm s t Eq_st =>
+       eq_ind s (fun t' => ren_Tm f_Tm s = ren_Tm g_Tm t')
+         (extRen_Tm f_Tm g_Tm Eq_Tm s) t Eq_st).
+Qed.
+
+#[global]
+Instance ren_Tm_morphism2 :
+ (Proper (respectful (pointwise_relation _ eq) (pointwise_relation _ eq))
+    (@ren_Tm)).
+Proof.
+exact (fun f_Tm g_Tm Eq_Tm s => extRen_Tm f_Tm g_Tm Eq_Tm s).
 Qed.
 
 Ltac auto_unfold := repeat
-                     unfold VarInstance_Term, Var, ids, Ren_Term, Ren1, ren1,
-                      Up_Term_Term, Up_Term, up_Term, Subst_Term, Subst1,
-                      subst1.
+                     unfold VarInstance_Tm, Var, ids, Ren_Tm, Ren1, ren1,
+                      Up_Tm_Tm, Up_Tm, up_Tm, Subst_Tm, Subst1, subst1,
+                      VarInstance_Ty, Var, ids, Ren_Ty, Ren1, ren1, Up_Ty_Ty,
+                      Up_Ty, up_Ty, Subst_Ty, Subst1, subst1.
 
 Tactic Notation "auto_unfold" "in" "*" := repeat
-                                           unfold VarInstance_Term, Var, ids,
-                                            Ren_Term, Ren1, ren1,
-                                            Up_Term_Term, Up_Term, up_Term,
-                                            Subst_Term, Subst1, subst1 
-                                            in *.
+                                           unfold VarInstance_Tm, Var, ids,
+                                            Ren_Tm, Ren1, ren1, Up_Tm_Tm,
+                                            Up_Tm, up_Tm, Subst_Tm, Subst1,
+                                            subst1, VarInstance_Ty, Var, ids,
+                                            Ren_Ty, Ren1, ren1, Up_Ty_Ty,
+                                            Up_Ty, up_Ty, Subst_Ty, Subst1,
+                                            subst1 in *.
 
 Ltac asimpl' := repeat (first
-                 [ progress setoid_rewrite substSubst_Term_pointwise
-                 | progress setoid_rewrite substSubst_Term
-                 | progress setoid_rewrite substRen_Term_pointwise
-                 | progress setoid_rewrite substRen_Term
-                 | progress setoid_rewrite renSubst_Term_pointwise
-                 | progress setoid_rewrite renSubst_Term
-                 | progress setoid_rewrite renRen'_Term_pointwise
-                 | progress setoid_rewrite renRen_Term
-                 | progress setoid_rewrite varLRen'_Term_pointwise
-                 | progress setoid_rewrite varLRen'_Term
-                 | progress setoid_rewrite varL'_Term_pointwise
-                 | progress setoid_rewrite varL'_Term
-                 | progress setoid_rewrite rinstId'_Term_pointwise
-                 | progress setoid_rewrite rinstId'_Term
-                 | progress setoid_rewrite instId'_Term_pointwise
-                 | progress setoid_rewrite instId'_Term
-                 | progress unfold up_Term_Term, upRen_Term_Term, up_ren
-                 | progress cbn[subst_Term ren_Term]
+                 [ progress setoid_rewrite substSubst_Ty_pointwise
+                 | progress setoid_rewrite substSubst_Ty
+                 | progress setoid_rewrite substRen_Ty_pointwise
+                 | progress setoid_rewrite substRen_Ty
+                 | progress setoid_rewrite renSubst_Ty_pointwise
+                 | progress setoid_rewrite renSubst_Ty
+                 | progress setoid_rewrite renRen'_Ty_pointwise
+                 | progress setoid_rewrite renRen_Ty
+                 | progress setoid_rewrite substSubst_Tm_pointwise
+                 | progress setoid_rewrite substSubst_Tm
+                 | progress setoid_rewrite substRen_Tm_pointwise
+                 | progress setoid_rewrite substRen_Tm
+                 | progress setoid_rewrite renSubst_Tm_pointwise
+                 | progress setoid_rewrite renSubst_Tm
+                 | progress setoid_rewrite renRen'_Tm_pointwise
+                 | progress setoid_rewrite renRen_Tm
+                 | progress setoid_rewrite varLRen'_Ty_pointwise
+                 | progress setoid_rewrite varLRen'_Ty
+                 | progress setoid_rewrite varL'_Ty_pointwise
+                 | progress setoid_rewrite varL'_Ty
+                 | progress setoid_rewrite rinstId'_Ty_pointwise
+                 | progress setoid_rewrite rinstId'_Ty
+                 | progress setoid_rewrite instId'_Ty_pointwise
+                 | progress setoid_rewrite instId'_Ty
+                 | progress setoid_rewrite varLRen'_Tm_pointwise
+                 | progress setoid_rewrite varLRen'_Tm
+                 | progress setoid_rewrite varL'_Tm_pointwise
+                 | progress setoid_rewrite varL'_Tm
+                 | progress setoid_rewrite rinstId'_Tm_pointwise
+                 | progress setoid_rewrite rinstId'_Tm
+                 | progress setoid_rewrite instId'_Tm_pointwise
+                 | progress setoid_rewrite instId'_Tm
+                 | progress
+                    unfold up_Ty_Ty, upRen_Ty_Ty, up_Tm_Tm, upRen_Tm_Tm,
+                     up_ren
+                 | progress cbn[subst_Ty ren_Ty subst_Tm ren_Tm]
                  | progress fsimpl ]).
 
 Ltac asimpl := check_no_evars;
                 repeat
-                 unfold VarInstance_Term, Var, ids, Ren_Term, Ren1, ren1,
-                  Up_Term_Term, Up_Term, up_Term, Subst_Term, Subst1, subst1
-                  in *; asimpl'; minimize.
+                 unfold VarInstance_Tm, Var, ids, Ren_Tm, Ren1, ren1,
+                  Up_Tm_Tm, Up_Tm, up_Tm, Subst_Tm, Subst1, subst1,
+                  VarInstance_Ty, Var, ids, Ren_Ty, Ren1, ren1, Up_Ty_Ty,
+                  Up_Ty, up_Ty, Subst_Ty, Subst1, subst1 in *; asimpl';
+                minimize.
 
 Tactic Notation "asimpl" "in" hyp(J) := revert J; asimpl; intros J.
 
 Tactic Notation "auto_case" := auto_case ltac:(asimpl; cbn; eauto).
 
-Ltac substify := auto_unfold; try setoid_rewrite rinstInst'_Term_pointwise;
-                  try setoid_rewrite rinstInst'_Term.
+Ltac substify := auto_unfold; try setoid_rewrite rinstInst'_Ty_pointwise;
+                  try setoid_rewrite rinstInst'_Ty;
+                  try setoid_rewrite rinstInst'_Tm_pointwise;
+                  try setoid_rewrite rinstInst'_Tm.
 
-Ltac renamify := auto_unfold;
-                  try setoid_rewrite_left rinstInst'_Term_pointwise;
-                  try setoid_rewrite_left rinstInst'_Term.
+Ltac renamify := auto_unfold; try setoid_rewrite_left rinstInst'_Ty_pointwise;
+                  try setoid_rewrite_left rinstInst'_Ty;
+                  try setoid_rewrite_left rinstInst'_Tm_pointwise;
+                  try setoid_rewrite_left rinstInst'_Tm.
 
 End Core.
 
@@ -622,9 +986,13 @@ Module Extra.
 
 Import Core.
 
-#[global]Hint Opaque subst_Term: rewrite.
+#[global]Hint Opaque subst_Ty: rewrite.
 
-#[global]Hint Opaque ren_Term: rewrite.
+#[global]Hint Opaque ren_Ty: rewrite.
+
+#[global]Hint Opaque subst_Tm: rewrite.
+
+#[global]Hint Opaque ren_Tm: rewrite.
 
 End Extra.
 
