theories/par.v
@@ -5,35 +5,51 @@ Import Ltac2.Constr.Unsafe.
 Require Ltac2.Control.
 Set Default Proof Mode "Classic".
 
+Inductive TyPar : Ty -> Ty -> Prop :=
+| TP_Var i :
+  TyPar (VarTy i) (VarTy i)
+| TP_Abs A0 A1 a0 a1 :
+  TyPar A0 A1 ->
+  TyPar a0 a1 ->
+  (* ------------------- *)
+  TyPar (TyAbs a0) (TyAbs a1)
+| TP_App b0 b1 a0 a1 :
+  TyPar b0 b1 ->
+  TyPar a0 a1 ->
+  (* ---------------------------- *)
+  TyPar (TyApp b0 a0) (TyApp b1 a1)
+| TP_AppAbs b0 b1 a0 a1 :
+  TyPar b0 b1 ->
+  TyPar a0 a1 ->
+  (* ---------------------------- *)
+  TyPar (TyApp (TyAbs b0) a0) (subst_Ty (a1…) b1).
+
+
 Reserved Infix "⇒" (at level 70, no associativity).
-Inductive Par : Term -> Term -> Prop :=
+Inductive Par : Tm -> Tm -> Prop :=
 | P_Var i :
   VarTm i ⇒ VarTm i
-| P_Sort s :
-  ISort s ⇒ ISort s
-| P_Abs A0 A1 a0 a1 :
-  A0 ⇒ A1 ->
+| P_Abs a0 a1 :
   a0 ⇒ a1 ->
   (* ------------------- *)
-  Abs A0 a0 ⇒ Abs A1 a1
-| P_Pi A0 A1 B0 B1 :
-  A0 ⇒ A1 ->
-  B0 ⇒ B1 ->
-  (* ------------------- *)
-  Pi A0 B0 ⇒ Pi A1 B1
+  TmAbs a0 ⇒ TmAbs a1
 | P_App a0 a1 b0 b1 :
   a0 ⇒ a1 ->
   b0 ⇒ b1 ->
-  App a0 b0 ⇒ App a1 b1
-| P_AppAbs A a0 a1 b0 b1 :
+  TmApp a0 b0 ⇒ TmApp a1 b1
+| P_AppAbs a0 a1 b0 b1 :
   a0 ⇒ a1 ->
   b0 ⇒ b1 ->
-  (* -------------------- *)
-  App (Abs A a0) b0 ⇒ a1[b1…]
+  (* ---------------------------------- *)
+  TmApp (TmAbs a0) b0 ⇒ subst_Tm (b1…) a1
+(* | P_Forall a0 a1 : *)
+(*   a0 ⇒ a1 -> *)
+(*   (* ------------------------------- *) *)
+(*   TmForall a0 ⇒ TmForall a1 *)
 
 where "a ⇒ b" := (Par a b).
 
-#[export]Hint Constructors Par : par.
+#[export]Hint Constructors Par TyPar : par.
 
 Infix "⇒*" := (rtc Par) (at level 70, no associativity).
 
@@ -111,7 +127,7 @@ Ltac2 par_cong_rel c r :=
 Ltac revert_all_terms :=
   repeat (progress
             (match goal with
-               [_x : Term |- _] => (revert _x)
+               [_x : Tm |- _] => (revert _x)
              end)).
 
 Ltac2 Notation "gen_cong" x(constr) r(constr) := Control.refine (fun _ => par_cong_rel x r).
@@ -130,23 +146,17 @@ Ltac solve_pars_cong :=
 Lemma PS_App : ltac2:(gen_cong P_App (rtc Par)).
 Proof. solve_pars_cong. Qed.
 
-Lemma PS_Pi : ltac2:(gen_cong P_Pi (rtc Par)).
-Proof. solve_pars_cong. Qed.
-
-Lemma PS_Sort : ltac2:(gen_cong P_Sort (rtc Par)).
-Proof. solve_pars_cong. Qed.
-
-Lemma P_AppAbs' A a0 a1 b0 b1 u :
-  u = a1[b1…] ->
+Lemma P_AppAbs' a0 a1 b0 b1 u :
+  u = subst_Tm (b1…) a1 ->
   a0 ⇒ a1 ->
   b0 ⇒ b1 ->
   (* -------------------- *)
-  App (Abs A a0) b0 ⇒ u.
+  TmApp (TmAbs a0) b0 ⇒ u.
 Proof. move =>> ->. apply P_AppAbs. Qed.
 
 Lemma par_renaming a b ξ :
   a ⇒ b ->
-  a⟨ξ⟩ ⇒ b⟨ξ⟩.
+  ren_Tm ξ a ⇒ ren_Tm ξ b.
 Proof.
   move => h. move : ξ. elim : a b/h => //=; eauto with par.
   (* Abs *)
@@ -165,13 +175,13 @@ Proof. eauto using par_refl. Qed.
 
 Lemma par_ρ_up ρ0 ρ1 :
   (forall i, ρ0 i ⇒ ρ1 i) ->
-  (forall i, (up_Term_Term ρ0) i ⇒ (up_Term_Term ρ1) i).
-Proof. hauto l:on use:par_renaming, par_ρ_ext, P_Var unfold:up_Term_Term. Qed.
+  (forall i, (up_Tm_Tm ρ0) i ⇒ (up_Tm_Tm ρ1) i).
+Proof. hauto l:on use:par_renaming, par_ρ_ext, P_Var unfold:up_Tm_Tm. Qed.
 
 Lemma par_morphing a b ρ0 ρ1 :
   (forall i, ρ0 i ⇒ ρ1 i) ->
   a ⇒ b ->
-  a[ρ0] ⇒ b[ρ1].
+  subst_Tm ρ0 a ⇒ subst_Tm ρ1 b.
 Proof.
   move => + h. move : ρ0 ρ1.
   elim : a b /h=>//=; eauto using par_ρ_up with par.
@@ -183,7 +193,7 @@ Qed.
 Lemma pars_morphing a b ρ0 ρ1 :
   (forall i, ρ0 i ⇒ ρ1 i) ->
   a ⇒* b ->
-  a[ρ0] ⇒* b[ρ1].
+  subst_Tm ρ0 a ⇒* subst_Tm ρ1 b.
 Proof.
   move => h.
   move => h0.
@@ -193,16 +203,15 @@ Qed.
 
 Function tstar a :=
   match a with
-  | ISort _ => a
   | VarTm _ => a
-  | Abs A a => Abs (tstar A) (tstar a)
-  | Pi A B => Pi (tstar A) (tstar B)
-  | App (Abs A a) b => (tstar a)[tstar b …]
-  | App a b => App (tstar a) (tstar b)
+  | TmAbs a => TmAbs (tstar a)
+  | TmApp (TmAbs a) b => subst_Tm (tstar b …)(tstar a)
+  | TmApp a b => TmApp (tstar a) (tstar b)
+  (* | TmForall a => TmForall (tstar a) *)
   end.
 
 Lemma par_cong a0 a1 b0 b1 (h : a0 ⇒ a1) (h1 : b0 ⇒ b1) :
-  a0 [b0…] ⇒ a1 [b1…].
+  subst_Tm (b0…) a0 ⇒ subst_Tm (b1…) a1.
 Proof. auto using par_morphing, par_ρ_ext, par_ρ_id. Qed.
 
 Local Ltac solve_triangle := qauto use:par_refl, par_cong ctrs:Par inv:Par.
@@ -223,21 +232,21 @@ Qed.
 
 Lemma pars_renaming a b ξ :
   a ⇒* b ->
-  a⟨ξ⟩ ⇒* b⟨ξ⟩.
+  ren_Tm ξ a ⇒* ren_Tm ξ b.
 Proof.
   induction 1; hauto lq:on ctrs:rtc use:par_renaming.
 Qed.
 
 Lemma par_subst a b ρ :
   a ⇒ b ->
-  a[ρ] ⇒ b[ρ].
+  subst_Tm ρ a ⇒ subst_Tm ρ b.
 Proof.
   auto using par_refl, par_morphing.
 Qed.
 
 Lemma pars_subst a b ρ :
   a ⇒* b ->
-  a[ρ] ⇒* b[ρ].
+  subst_Tm ρ a ⇒* subst_Tm ρ b.
 Proof.
   induction 1; hauto lq:on ctrs:rtc use:par_subst.
 Qed.
@@ -248,12 +257,12 @@ Infix "⇔" := Coherent (at level 70, no associativity).
 
 Lemma coherent_renaming a b ξ :
   a ⇔ b ->
-  a⟨ξ⟩ ⇔ b⟨ξ⟩.
+  ren_Tm ξ a ⇔ ren_Tm ξ b.
 Proof. hauto lq:on use:pars_renaming unfold:Coherent. Qed.
 
 Lemma coherent_subst a b ρ :
   a ⇔ b ->
-  a[ρ] ⇔ b[ρ].
+  subst_Tm ρ a ⇔ subst_Tm ρ b.
 Proof. hauto lq:on use:pars_subst unfold:Coherent. Qed.
 
 Lemma coherent_refl : forall a, a ⇔ a.
@@ -274,63 +283,60 @@ Qed.
 Lemma C_App : ltac2:(gen_cong P_App Coherent).
 Proof. hauto lq:on use:PS_App unfold:Coherent. Qed.
 
-Lemma C_Pi : ltac2:(gen_cong P_Pi Coherent).
-Proof. hauto lq:on use:PS_Pi unfold:Coherent. Qed.
+(* Lemma pars_pi_inv A B U : *)
+(*   Pi A B ⇒* U -> exists A0 B0, U = Pi A0 B0 /\ A ⇒* A0 /\ B ⇒* B0. *)
+(* Proof. *)
+(*   move E : (Pi A B) => T h. *)
+(*   move : A B E. *)
+(*   elim : T U/h. *)
+(*   hauto lq:on ctrs:rtc, Par. *)
+(*   hauto lq:on rew:off inv:Par ctrs:Par,rtc. *)
+(* Qed. *)
 
-Lemma pars_pi_inv A B U :
-  Pi A B ⇒* U -> exists A0 B0, U = Pi A0 B0 /\ A ⇒* A0 /\ B ⇒* B0.
-Proof.
-  move E : (Pi A B) => T h.
-  move : A B E.
-  elim : T U/h.
-  hauto lq:on ctrs:rtc, Par.
-  hauto lq:on rew:off inv:Par ctrs:Par,rtc.
-Qed.
+(* Lemma pars_sort_inv s U : *)
+(*   ISort s ⇒* U -> U = ISort s. *)
+(* Proof. *)
+(*   move E : (ISort s) => T h. *)
+(*   move : s E. *)
+(*   elim : T U/h. *)
+(*   hauto lq:on ctrs:rtc, Par. *)
+(*   hauto lq:on rew:off inv:Par ctrs:Par,rtc. *)
+(* Qed. *)
 
-Lemma pars_sort_inv s U :
-  ISort s ⇒* U -> U = ISort s.
-Proof.
-  move E : (ISort s) => T h.
-  move : s E.
-  elim : T U/h.
-  hauto lq:on ctrs:rtc, Par.
-  hauto lq:on rew:off inv:Par ctrs:Par,rtc.
-Qed.
+(* Lemma coherent_pi_inj A0 A1 B0 B1 : *)
+(*   Pi A0 B0 ⇔ Pi A1 B1 -> *)
+(*   A0 ⇔ A1 /\ *)
+(*   B0 ⇔ B1. *)
+(* Proof. hauto l:on inv:eq rew:off  ctrs:rtc use:pars_pi_inv unfold:Coherent. Qed. *)
 
-Lemma coherent_pi_inj A0 A1 B0 B1 :
-  Pi A0 B0 ⇔ Pi A1 B1 ->
-  A0 ⇔ A1 /\
-  B0 ⇔ B1.
-Proof. hauto l:on inv:eq rew:off  ctrs:rtc use:pars_pi_inv unfold:Coherent. Qed.
-
-Lemma coherent_sort_inj s0 s1 :
-  ISort s0 ⇔ ISort s1 ->
-  s0 = s1.
-Proof.
-  move => [u][/pars_sort_inv h0 /pars_sort_inv h1].
-  congruence.
-Qed.
+(* Lemma coherent_sort_inj s0 s1 : *)
+(*   ISort s0 ⇔ ISort s1 -> *)
+(*   s0 = s1. *)
+(* Proof. *)
+(*   move => [u][/pars_sort_inv h0 /pars_sort_inv h1]. *)
+(*   congruence. *)
+(* Qed. *)
 
 (* Based on https://poplmark-reloaded.github.io/coq/well-scoped/PR.sn_defs.html *)
-Inductive SN : Term -> Prop :=
-| S_Neu a : SNe a -> SN a
-| S_Abs A a : SN A -> SN a -> SN (Abs A a)
-| S_Sort s : SN (ISort s)
-| S_Pi A B : SN A -> SN B -> SN (Pi A B)
-| S_Red a0 a1 : SNRed a0 a1 -> SN a1 -> SN a0
-with SNe : Term -> Prop :=
-| S_Var i : SNe (VarTm i)
-| S_App a b : SNe a -> SN b -> SNe (App a b)
-with SNRed : Term -> Term -> Prop :=
-| S_AppL a0 a1 b :
-  SNRed a0 a1 ->
-  SNRed (App a0 b) (App a1 b)
-| S_AppAbs A a b :
-  SN A ->
-  SN b ->
-  SNRed (App (Abs A a) b) a[b…].
+(* Inductive SN : Term -> Prop := *)
+(* | S_Neu a : SNe a -> SN a *)
+(* | S_Abs A a : SN A -> SN a -> SN (Abs A a) *)
+(* | S_Sort s : SN (ISort s) *)
+(* | S_Pi A B : SN A -> SN B -> SN (Pi A B) *)
+(* | S_Red a0 a1 : SNRed a0 a1 -> SN a1 -> SN a0 *)
+(* with SNe : Term -> Prop := *)
+(* | S_Var i : SNe (VarTm i) *)
+(* | S_App a b : SNe a -> SN b -> SNe (App a b) *)
+(* with SNRed : Term -> Term -> Prop := *)
+(* | S_AppL a0 a1 b : *)
+(*   SNRed a0 a1 -> *)
+(*   SNRed (App a0 b) (App a1 b) *)
+(* | S_AppAbs A a b : *)
+(*   SN A -> *)
+(*   SN b -> *)
+(*   SNRed (App (Abs A a) b) a[b…]. *)
 
-Scheme SN_ind_2 := Minimality for SN Sort Prop
-                   with SNe_ind_2 := Minimality for SNe Sort Prop
-                    with redSN_ind_2 := Minimality for SNRed Sort Prop.
-Combined Scheme SN_multind from SN_ind_2, SNe_ind_2, redSN_ind_2.
+(* Scheme SN_ind_2 := Minimality for SN Sort Prop *)
+(*                    with SNe_ind_2 := Minimality for SNe Sort Prop *)
+(*                     with redSN_ind_2 := Minimality for SNRed Sort Prop. *)
+(* Combined Scheme SN_multind from SN_ind_2, SNe_ind_2, redSN_ind_2. *)
